thys/Real_Time_Deque/Stack_Aux.thy
@@ -2,6 +2,8 @@ theory Stack_Aux
 imports Stack
 begin
 
+text\<open>The function \<open>list\<close> appends the two lists and is needed for the list abstraction of the deque.\<close>
+
 fun list :: "'a stack \<Rightarrow> 'a list" where
   "list (Stack left right) = left @ right"
 
